

# SUMS OF POWERS VIA CENTRAL FINITE DIFFERENCES AND NEWTON'S FORMULA

PETRO KOLOSOV

ABSTRACT.

## 1. INTRODUCTION AND MAIN RESULTS

**Theorem 1.1** (Newton series via central difference).

$$f(x) = \sum_{k=0}^{\infty} \frac{x^{[k]}}{k!} \delta^k f(0)$$

**Theorem 1.2** (Newton series for power via central difference).

$$x^n = \sum_{k=0}^{\infty} \frac{x^{[k]}}{k!} \delta^k 0^n$$

Where

**Corollary 1.3** (Central difference of power in zero).

$$\delta^k 0^n = \sum_{j=0}^k (-1)^j \binom{k}{j} \left( \frac{k}{2} - j \right)^n$$

**Lemma 1.4** (Central factorial).

$$n^{[k]} = n \left( n + \frac{k}{2} - 1 \right) \left( n + \frac{k}{2} - 2 \right) \cdots \left( n - \frac{k}{2} + 1 \right) = n \prod_{j=1}^{k-1} \left( n + \frac{k}{2} - j \right)$$

Such that

**Proposition 1.5.**

$$n^{[k]} = n \left( n + \frac{k}{2} - 1 \right)_{k-1}$$

---

*Date:* December 29, 2025.

2010 *Mathematics Subject Classification.* 05A19, 05A10, 11B73, 11B83.

**Proposition 1.6.** *For  $k \geq 1$*

$$\begin{aligned} \frac{n^{[k]}}{k!} &= \frac{1}{k!} n \left( n + \frac{k}{2} - 1 \right)_{k-1} = \frac{n}{k(k-1)!} \left( n + \frac{k}{2} - 1 \right)_{k-1} \\ &= \frac{n}{k} \binom{n + \frac{k}{2} - 1}{k-1} \end{aligned}$$

Because

**Proposition 1.7.**

$$\frac{(x)_n}{n!} = \binom{x}{n}$$

Thus

**Proposition 1.8.**

$$x^n = \sum_{k=1}^n \frac{x}{k} \binom{x + \frac{k}{2} - 1}{k-1} \delta^k 0^n$$

We start from  $k = 1$  there because for all  $k = 0$  the central difference  $\delta^k 0^n$  is zero.

Thus

**Proposition 1.9.**

$$x^{n-1} = \sum_{k=1}^n \frac{1}{k} \binom{x + \frac{k}{2} - 1}{k-1} \delta^k 0^n$$

Thus

**Proposition 1.10.**

$$x^n = \sum_{k=0}^n \frac{1}{k+1} \binom{x + \frac{k+1}{2} - 1}{k} \delta^{k+1} 0^{n+1}$$

Thus

**Proposition 1.11.**

$$\sum^r n^m = \sum_{k=0}^m \frac{1}{k+1} \binom{n + \frac{k+1}{2} - 1 + r}{k+r} \delta^{k+1} 0^{m+1}$$

*Proof.* By hockey stick identity. □

**Lemma 1.12** (Central factorial numbers).

$$\delta^k 0^n = k! T(n, k)$$

Thus

**Proposition 1.13.**

$$\sum^r n^m = \sum_{k=0}^m \frac{1}{k+1} \binom{n + \frac{k+1}{2} - 1 + r}{k+r} (k+1)! T(m+1, k+1)$$

Thus

**Proposition 1.14.**

$$\sum^r n^{m-1} = \sum_{k=0}^m k! \binom{n + \frac{k+1}{2} - 1 + r}{k+r} T(m, k+1)$$

## 2. PROOF OF KNUTH'S FORMULA

## 3. CONCLUSIONS

## 4. ACKNOWLEDGEMENTS

The author is grateful to [Full Name] for his valuable contribution [contribution] about the fact that [interesting claim].

**Version:** Local-0.1.0

**License:** This work is licensed under a [CC BY 4.0 License](#).

**Sources:** [github.com/kolosovpetro/SumsOfPowersViaCentralFiniteDifferencesAndNewtonFormula](https://github.com/kolosovpetro/SumsOfPowersViaCentralFiniteDifferencesAndNewtonFormula)

**ORCID:** [0000-0002-6544-8880](#)

**Email:** [kolosovp94@gmail.com](mailto:kolosovp94@gmail.com)